src/ReactorModel/Objects/Reactor/Core.lean
@@ -48,55 +48,55 @@ abbrev «with»
   Reactor.Core.mk ports acts state rcns nest
 
 def insert [inst : ReactorType Reactor.Core] 
-    (rtr : Reactor.Core) (cmp : Component) (i : ID) (v : inst.componentType cmp) :=
-  match cmp with
+    (rtr : Reactor.Core) (cpt : Component) (i : ID) (v : inst.componentType cpt) :=
+  match cpt with
   | .prt k => rtr.with (ports := Function.update (ports rtr) k $ ports rtr k |>.insert i v)
   | .act   => rtr.with (acts  := acts  rtr |>.insert i v)
   | .stv   => rtr.with (state := state rtr |>.insert i v)
   | .rcn   => rtr.with (rcns  := rcns  rtr |>.insert i v)
   | .rtr   => rtr.with (nest  := nest  rtr |>.insert i v)
 
-theorem insert_cmp?_eq_self {rtr : Reactor.Core} (cmp) {i v} : 
-    cmp? cmp (rtr.insert cmp i v) i = v := by
-  cases cmp <;> try cases ‹Component.Valued› 
+theorem insert_cpt?_eq_self {rtr : Reactor.Core} (cpt) {i v} : 
+    cpt? cpt (rtr.insert cpt i v) i = v := by
+  cases cpt <;> try cases ‹Component.Valued› 
   all_goals
-    simp [insert, cmp?, reactorType]
+    simp [insert, cpt?, reactorType]
     apply Partial.insert_same
 
-theorem insert_cmp?_ne_cmp_or_id {rtr : Reactor.Core} {cmp v} (h : c ≠ cmp ∨ j ≠ i) :
-    cmp? c rtr j = cmp? c (rtr.insert cmp i v) j := by
-  cases cmp <;> try cases ‹Component.Valued› <;> try cases ‹Kind›
+theorem insert_cpt?_ne_cpt_or_id {rtr : Reactor.Core} (h : c ≠ cpt ∨ j ≠ i) :
+    cpt? c rtr j = cpt? c (rtr.insert cpt i v) j := by
+  cases cpt <;> try cases ‹Component.Valued› <;> try cases ‹Kind›
   all_goals cases c <;> try cases ‹Component.Valued› <;> try cases ‹Kind›
   all_goals 
-    simp [cmp?, insert]
+    simp [cpt?, insert]
     try simp [reactorType]; done
   all_goals
     cases h
     case inl h => contradiction
     case inr h => exact Partial.insert_ne _ h |>.symm
 
-def updateMem {rtr : Reactor.Core} {cmp : Component.Valued} (f : cmp.type → cmp.type) : 
-    Member cmp i rtr → Reactor.Core
-  | .final h           => rtr.insert cmp i $ f (Partial.mem_ids_iff.mp h).choose
+def updateMem {rtr : Reactor.Core} {cpt : Component.Valued} (f : cpt.type → cpt.type) : 
+    Member cpt i rtr → Reactor.Core
+  | .final h           => rtr.insert cpt i $ f (Partial.mem_ids_iff.mp h).choose
   | .nest (j := j) _ l => rtr.insert .rtr j (updateMem f l)
 
 theorem updateMem_lawfulMemUpdate 
-    {cmp : Component.Valued} (l : Member cmp i rtr) 
-    (f : cmp.type → cmp.type) : LawfulMemUpdate cmp i f rtr (updateMem f l) := by
+    {cpt : Component.Valued} (l : Member cpt i rtr) 
+    (f : cpt.type → cpt.type) : LawfulMemUpdate cpt i f rtr (updateMem f l) := by
   induction l <;> simp [updateMem] 
   case final h =>
     replace h := Partial.mem_ids_iff.mp h
-    exact .final insert_cmp?_ne_cmp_or_id h.choose_spec (insert_cmp?_eq_self cmp)
+    exact .final insert_cpt?_ne_cpt_or_id h.choose_spec (insert_cpt?_eq_self cpt)
   case nest h l hi =>
-    exact .nest insert_cmp?_ne_cmp_or_id h (insert_cmp?_eq_self .rtr) hi
+    exact .nest insert_cpt?_ne_cpt_or_id h (insert_cpt?_eq_self .rtr) hi
 
-def update (rtr : Reactor.Core) (cmp : Component.Valued) (i : ID) (f : cmp.type → cmp.type) :=
-  if l : Nonempty (Member cmp i rtr) then updateMem f l.some else rtr
+def update (rtr : Reactor.Core) (cpt : Component.Valued) (i : ID) (f : cpt.type → cpt.type) :=
+  if l : Nonempty (Member cpt i rtr) then updateMem f l.some else rtr
 
 instance : ReactorType.LawfulUpdatable Reactor.Core where
   update := update
-  lawful rtr cmp i f := 
-    if h : Nonempty (Member (Component.val cmp) i rtr) 
+  lawful rtr cpt i f := 
+    if h : Nonempty (Member (Component.val cpt) i rtr) 
     then .update $ by simp [update, h]; exact updateMem_lawfulMemUpdate h.some f
     else .notMem (not_nonempty_iff.mp h) $ by simp [update, h]
 
