src/ReactorModel/Objects/Reactor/ReactorType/Indexable.lean
@@ -5,7 +5,7 @@ open Reactor (Component)
 namespace ReactorType
 
 def UniqueIDs [ReactorType α] (rtr : α) : Prop :=
-  ∀ {cmp i}, Subsingleton (Member cmp i rtr)
+  ∀ {cpt i}, Subsingleton (Member cpt i rtr)
 
 theorem UniqueIDs.lift [ReactorType α] [ReactorType β] [LawfulCoe α β] {rtr : α} 
     (h : UniqueIDs (rtr : β)) : UniqueIDs rtr where
@@ -14,8 +14,8 @@ theorem UniqueIDs.lift [ReactorType α] [ReactorType β] [LawfulCoe α β] {rtr 
       |>.trans (Member.Equivalent.from_lawfulCoe m₂).symm 
       |>.to_eq
 
-theorem UniqueIDs.updated [ReactorType.WellFounded α] {rtr₁ rtr₂ : α} {cmp i f} 
-    (u : LawfulUpdate cmp i f rtr₁ rtr₂) (h : UniqueIDs rtr₁) : UniqueIDs rtr₂ where
+theorem UniqueIDs.updated [ReactorType.WellFounded α] {rtr₁ rtr₂ : α}
+    (u : LawfulUpdate cpt i f rtr₁ rtr₂) (h : UniqueIDs rtr₁) : UniqueIDs rtr₂ where
   allEq m₁ m₂ := open Member in
     h.allEq (.fromLawfulUpdate m₁ u) (.fromLawfulUpdate m₂ u) ▸ Equivalent.from_lawfulUpdate u m₁ 
       |>.trans (Equivalent.from_lawfulUpdate u m₂).symm 
@@ -26,21 +26,21 @@ class Indexable (α) extends LawfulUpdatable α where
 
 namespace Member
 
-variable [LawfulUpdatable α] {cmp}
+variable [LawfulUpdatable α]
 
-def container {rtr : α} : Member cmp i rtr → Identified α
+def container {rtr : α} : Member cpt i rtr → Identified α
   | .nest _ (.nest h l)             => container (.nest h l)
   | .nest (rtr₂ := con) (j := j) .. => { id := j, obj := con }
   | .final _                        => { id := ⊤, obj := rtr }
 
 theorem nest_container  {rtr₁ rtr₂ : α} 
-    (h : ReactorType.nest rtr₁ i = some rtr₂) (m : Member cmp j rtr₂) : 
+    (h : ReactorType.nest rtr₁ i = some rtr₂) (m : Member cpt j rtr₂) : 
     ∃ (k : ID) (con : α), (Member.nest h m).container = ⟨k, con⟩ := by
   induction m generalizing i rtr₁
   case final => simp [container]
   case nest hn _ hi => simp [container, hi hn]
 
-theorem container_eq_root {rtr : α} {m : Member cmp i rtr} (h : m.container = ⟨⊤, con⟩) : 
+theorem container_eq_root {rtr : α} {m : Member cpt i rtr} (h : m.container = ⟨⊤, con⟩) : 
     rtr = con := by
   induction m generalizing con
   case final => 
@@ -58,50 +58,50 @@ instance [LawfulUpdatable α] [ind : Indexable β] [LawfulCoe α β] : Indexable
   unique_ids := UniqueIDs.lift ind.unique_ids 
 
 open Classical in
-noncomputable def con? [Indexable α] (rtr : α) (cmp : Component) : ID ⇀ Identified α := 
-  fun i => if m : Nonempty (Member cmp i rtr) then m.some.container else none
+noncomputable def con? [Indexable α] (rtr : α) (cpt : Component) : ID ⇀ Identified α := 
+  fun i => if m : Nonempty (Member cpt i rtr) then m.some.container else none
 
-notation rtr "[" cmp "]&"        => ReactorType.Indexable.con? rtr cmp
-notation rtr "[" cmp "][" i "]&" => ReactorType.Indexable.con? rtr cmp i
+notation rtr "[" cpt "]&"        => ReactorType.Indexable.con? rtr cpt
+notation rtr "[" cpt "][" i "]&" => ReactorType.Indexable.con? rtr cpt i
 
 noncomputable def obj? [a : Indexable α] (rtr : α) : 
-    (cmp : Component) → cmp.idType ⇀ a.componentType cmp
-  | .val cmp, i       => rtr[.val cmp][i]& >>= (cmp? (.val cmp) ·.obj i)
-  | .rcn,     i       => rtr[.rcn][i]&     >>= (cmp? .rcn       ·.obj i)
-  | .rtr,     .nest i => rtr[.rtr][i]&     >>= (cmp? .rtr       ·.obj i)
+    (cpt : Component) → cpt.idType ⇀ a.componentType cpt
+  | .val cpt, i       => rtr[.val cpt][i]& >>= (cpt? (.val cpt) ·.obj i)
+  | .rcn,     i       => rtr[.rcn][i]&     >>= (cpt? .rcn       ·.obj i)
+  | .rtr,     .nest i => rtr[.rtr][i]&     >>= (cpt? .rtr       ·.obj i)
   | .rtr,     ⊤       => rtr
 
-notation (priority := 1001) rtr "[" cmp "]" => ReactorType.Indexable.obj? rtr cmp
-notation rtr "[" cmp "][" i "]"             => ReactorType.Indexable.obj? rtr cmp i
+notation (priority := 1001) rtr "[" cpt "]" => ReactorType.Indexable.obj? rtr cpt
+notation rtr "[" cpt "][" i "]"             => ReactorType.Indexable.obj? rtr cpt i
 
-variable [a : Indexable α] {cmp : Component} {rtr rtr₁ : α}
+variable [a : Indexable α] {rtr rtr₁ : α}
 
-theorem con?_eq_some (h : rtr[cmp][i]& = some con) : 
-    ∃ m : Member cmp i rtr, m.container = con := by
+theorem con?_eq_some (h : rtr[cpt][i]& = some con) : 
+    ∃ m : Member cpt i rtr, m.container = con := by
   simp [con?] at h
   split at h
   case inl n => exists n.some; injection h
   case inr => contradiction
 
-theorem obj?_to_con?_and_cmp? {o} {i : ID} (h : rtr[cmp][i] = some o) :
-    ∃ c, (rtr[cmp][i]& = some c) ∧ (cmp? cmp c.obj i = some o) := by
-  cases cmp
+theorem obj?_to_con?_and_cpt? {o} {i : ID} (h : rtr[cpt][i] = some o) :
+    ∃ c, (rtr[cpt][i]& = some c) ∧ (cpt? cpt c.obj i = some o) := by
+  cases cpt
   all_goals 
     simp [obj?, bind] at h
     assumption
 
-theorem cmp?_to_con? {o} (h : cmp? cmp rtr i = some o) : rtr[cmp][i]& = some ⟨⊤, rtr⟩ := by
+theorem cpt?_to_con? {o} (h : cpt? cpt rtr i = some o) : rtr[cpt][i]& = some ⟨⊤, rtr⟩ := by
   let m := Member.final (Partial.mem_ids_iff.mpr ⟨_, h⟩)
   simp [con?, Nonempty.intro m, ←a.unique_ids.allEq m, Member.container]
 
-theorem cmp?_to_obj? {o} (h : cmp? cmp rtr i = some o) : rtr[cmp][i] = some o := by
-  cases cmp
+theorem cpt?_to_obj? {o} (h : cpt? cpt rtr i = some o) : rtr[cpt][i] = some o := by
+  cases cpt
   all_goals 
     simp [obj?, bind]
-    exact ⟨⟨⊤, rtr⟩, cmp?_to_con? h, h⟩ 
+    exact ⟨⟨⊤, rtr⟩, cpt?_to_con? h, h⟩ 
 
-theorem con?_nested {c : ID} (h : nest rtr₁ i = some rtr₂) (ho : rtr₂[cmp][j]& = some ⟨c, con⟩) : 
-    rtr₁[cmp][j]& = some ⟨c, con⟩ := by
+theorem con?_nested {c : ID} (h : nest rtr₁ i = some rtr₂) (ho : rtr₂[cpt][j]& = some ⟨c, con⟩) : 
+    rtr₁[cpt][j]& = some ⟨c, con⟩ := by
   simp [con?] at ho ⊢ 
   split at ho
   case inr => contradiction
@@ -115,15 +115,15 @@ theorem con?_nested {c : ID} (h : nest rtr₁ i = some rtr₂) (ho : rtr₂[cmp]
       simp [hm, Member.container] at ho
       simp [Nonempty.intro l₁, ←a.unique_ids.allEq l₁, Member.container, ho]
 
-theorem con?_eq_root (h : rtr[cmp][i]& = some ⟨⊤, con⟩) : rtr = con :=
+theorem con?_eq_root (h : rtr[cpt][i]& = some ⟨⊤, con⟩) : rtr = con :=
   Member.container_eq_root (con?_eq_some h).choose_spec
 
-theorem obj?_nested {o} {j : ID} (h : nest rtr₁ i = some rtr₂) (ho : rtr₂[cmp][j] = some o) : 
-    rtr₁[cmp][j] = some o := by
-  cases cmp <;> try cases j
+theorem obj?_nested {o} {j : ID} (h : nest rtr₁ i = some rtr₂) (ho : rtr₂[cpt][j] = some o) : 
+    rtr₁[cpt][j] = some o := by
+  cases cpt <;> try cases j
   all_goals
     simp [obj?, bind]
-    have ⟨⟨c, con⟩, hc, ho⟩ := obj?_to_con?_and_cmp? ho 
+    have ⟨⟨c, con⟩, hc, ho⟩ := obj?_to_con?_and_cpt? ho 
     cases c
     case nest c => 
       have := con?_nested h hc
@@ -140,34 +140,34 @@ theorem obj?_nested {o} {j : ID} (h : nest rtr₁ i = some rtr₂) (ho : rtr₂[
 theorem obj?_nested_root (h : nest rtr₁ i = some rtr₂) (ho : rtr₂[.rtr][⊤] = some rtr₃) : 
     ∃ j, rtr₁[.rtr][j] = some rtr₃ := by
   simp [obj?] at ho
-  exact ⟨i, ho ▸ cmp?_to_obj? h⟩
+  exact ⟨i, ho ▸ cpt?_to_obj? h⟩
 
 -- This is a version of `obj?_nested`, where we don't restrict `j` to be an `ID`. This makes a 
--- difference when `cmp = .rtr`. Note that if `cmp = .rtr` and `j = ⊤`, then `j' = .nest i`.
-theorem obj?_nested' {o j} (h : nest rtr₁ i = some rtr₂) (ho : rtr₂[cmp][j] = some o) : 
-    ∃ j', rtr₁[cmp][j'] = some o := by
-  cases cmp <;> try cases j
+-- difference when `cpt = .rtr`. Note that if `cpt = .rtr` and `j = ⊤`, then `j' = .nest i`.
+theorem obj?_nested' {o j} (h : nest rtr₁ i = some rtr₂) (ho : rtr₂[cpt][j] = some o) : 
+    ∃ j', rtr₁[cpt][j'] = some o := by
+  cases cpt <;> try cases j
   case rtr.root => exact obj?_nested_root h ho
   all_goals exact ⟨_, obj?_nested h ho⟩
 
-theorem obj?_mem_ids_nested {cmp : Component.Valued} 
-    (h : nest rtr₁ i = some rtr₂) (hm : j ∈ rtr₂[cmp].ids) : j ∈ rtr₁[cmp].ids :=
+theorem obj?_mem_ids_nested {cpt : Component.Valued} 
+    (h : nest rtr₁ i = some rtr₂) (hm : j ∈ rtr₂[cpt].ids) : j ∈ rtr₁[cpt].ids :=
   Partial.mem_ids_iff.mpr ⟨_, obj?_nested h (Partial.mem_ids_iff.mp hm).choose_spec⟩  
 
-theorem member_isEmpty_con?_none (h : IsEmpty (Member cmp i rtr)) : rtr[cmp][i]& = none := by
-  cases cmp <;> simp [con?, not_nonempty_iff.mpr h]
+theorem member_isEmpty_con?_none (h : IsEmpty (Member cpt i rtr)) : rtr[cpt][i]& = none := by
+  cases cpt <;> simp [con?, not_nonempty_iff.mpr h]
 
-theorem member_isEmpty_obj?_none (h : IsEmpty (Member cmp i rtr)) : rtr[cmp][i] = none := by
-  cases cmp <;> simp [obj?, member_isEmpty_con?_none h, bind]
+theorem member_isEmpty_obj?_none (h : IsEmpty (Member cpt i rtr)) : rtr[cpt][i] = none := by
+  cases cpt <;> simp [obj?, member_isEmpty_con?_none h, bind]
 
 end Indexable
 
 namespace LawfulCoe
 
-variable [a : Indexable α] [b : Indexable β] [c : LawfulCoe α β] {cmp : Component} {rtr : α}
+variable [a : Indexable α] [b : Indexable β] [c : LawfulCoe α β] {rtr : α}
 
-theorem lower_container_eq {m : Member cmp i rtr} (h : m.container = con) : 
-    (m : Member cmp i (rtr : β)).container = ↑con := by
+theorem lower_container_eq {m : Member cpt i rtr} (h : m.container = con) : 
+    (m : Member cpt i (rtr : β)).container = ↑con := by
   induction m
   case final =>
     simp [Member.container] at h ⊢
@@ -181,24 +181,24 @@ theorem lower_container_eq {m : Member cmp i rtr} (h : m.container = con) :
       simp [Member.container] at h
       simp [←hi h, Member.fromLawfulCoe, Member.container]
 
-theorem lower_con?_some (h : rtr[cmp][i]& = some con) : (rtr : β)[cmp][i]& = some ↑con := by
+theorem lower_con?_some (h : rtr[cpt][i]& = some con) : (rtr : β)[cpt][i]& = some ↑con := by
   simp [Indexable.con?] at h ⊢
   split at h
   case inr => contradiction 
   case inl n =>
     injection h with h
-    simp [←c.lower_container_eq h, (⟨n.some⟩ : Nonempty (Member cmp i (rtr : β)))]
+    simp [←c.lower_container_eq h, (⟨n.some⟩ : Nonempty (Member cpt i (rtr : β)))]
     congr
     apply b.unique_ids.allEq
 
-theorem lower_obj?_some {i o} (h : rtr[cmp][i] = some o) : (rtr : β)[cmp][i] = some ↑o := by
-  cases cmp <;> try cases i
+theorem lower_obj?_some {i o} (h : rtr[cpt][i] = some o) : (rtr : β)[cpt][i] = some ↑o := by
+  cases cpt <;> try cases i
   case rtr.root => simp_all [Indexable.obj?]
   all_goals
-    have ⟨_, h₁, h₂⟩ := a.obj?_to_con?_and_cmp? h
-    simp [Indexable.obj?, bind, c.lower_con?_some h₁, c.lower_cmp?_eq_some _ h₂]
+    have ⟨_, h₁, h₂⟩ := a.obj?_to_con?_and_cpt? h
+    simp [Indexable.obj?, bind, c.lower_con?_some h₁, c.lower_cpt?_eq_some _ h₂]
 
-theorem lower_mem_obj?_ids {i} (h : i ∈ rtr[cmp].ids) : i ∈ (rtr : β)[cmp].ids :=
+theorem lower_mem_obj?_ids {i} (h : i ∈ rtr[cpt].ids) : i ∈ (rtr : β)[cpt].ids :=
   Partial.mem_ids_iff.mpr ⟨_, c.lower_obj?_some (Partial.mem_ids_iff.mp h).choose_spec⟩ 
 
 end LawfulCoe
@@ -209,10 +209,10 @@ namespace LawfulMemUpdate
 
 variable [Indexable α] {rtr₁ : α}
 
-theorem obj?_preserved {cmp f} (u : LawfulMemUpdate cmp i f rtr₁ rtr₂) (h : c ≠ cmp ∨ j ≠ i) : 
+theorem obj?_preserved (u : LawfulMemUpdate cpt i f rtr₁ rtr₂) (h : c ≠ cpt ∨ j ≠ i) : 
     rtr₂[c][j] = rtr₁[c][j] := by
   -- TODO: We need to somehow distinguish whether [c][j] even identifies a component, and if so, 
-  --       whether it lives in the same reactor as [cmp][i].
+  --       whether it lives in the same reactor as [cpt][i].
   induction u
   case final e _ _ =>
     have := e (c := c) (j := j) (by simp [h])
@@ -220,23 +220,21 @@ theorem obj?_preserved {cmp f} (u : LawfulMemUpdate cmp i f rtr₁ rtr₂) (h : 
   case nest =>
     sorry
 
-theorem obj?_some₁ {cmp f} (u : LawfulMemUpdate cmp i f rtr₁ rtr₂) : 
-    ∃ o, rtr₁[cmp][i] = some o := by
+theorem obj?_some₁ (u : LawfulMemUpdate cpt i f rtr₁ rtr₂) : ∃ o, rtr₁[cpt][i] = some o := by
   induction u 
-  case final         => exact ⟨_, cmp?_to_obj? ‹_›⟩
+  case final         => exact ⟨_, cpt?_to_obj? ‹_›⟩
   case nest h _ _ hi => exact ⟨_, obj?_nested h hi.choose_spec⟩
 
-theorem obj?_some₂ {cmp f} (u : LawfulMemUpdate cmp i f rtr₁ rtr₂) : 
-    ∃ o, rtr₂[cmp][i] = some o := by
+theorem obj?_some₂ (u : LawfulMemUpdate cpt i f rtr₁ rtr₂) : ∃ o, rtr₂[cpt][i] = some o := by
   induction u 
-  case final       => exact ⟨_, cmp?_to_obj? ‹_›⟩
+  case final       => exact ⟨_, cpt?_to_obj? ‹_›⟩
   case nest h _ hi => exact ⟨_, obj?_nested h hi.choose_spec⟩
 
-theorem obj?_updated {cmp f} (u : LawfulMemUpdate cmp i f rtr₁ rtr₂) : 
-    rtr₂[cmp][i] = f <$> rtr₁[cmp][i] := by
+theorem obj?_updated (u : LawfulMemUpdate cpt i f rtr₁ rtr₂) : 
+    rtr₂[cpt][i] = f <$> rtr₁[cpt][i] := by
   induction u
   case final h₁ h₂ => 
-    rw [cmp?_to_obj? h₁, cmp?_to_obj? h₂, Option.map_some]
+    rw [cpt?_to_obj? h₁, cpt?_to_obj? h₂, Option.map_some]
   case nest h₁ h₂ u hi =>
     have ⟨_, h₁'⟩ := u.obj?_some₁
     have ⟨_, h₂'⟩ := u.obj?_some₂
@@ -249,12 +247,12 @@ namespace LawfulUpdate
 
 variable [Indexable α] {rtr₁ : α}
 
-theorem obj?_preserved {cmp f} (h : c ≠ cmp ∨ j ≠ i) : 
-    (LawfulUpdate cmp i f rtr₁ rtr₂) → rtr₂[c][j] = rtr₁[c][j]
+theorem obj?_preserved (h : c ≠ cpt ∨ j ≠ i) : 
+    (LawfulUpdate cpt i f rtr₁ rtr₂) → rtr₂[c][j] = rtr₁[c][j]
   | update u   => u.obj?_preserved h
   | notMem _ h => h ▸ rfl
 
-theorem obj?_updated {cmp f} : (LawfulUpdate cmp i f rtr₁ rtr₂) → rtr₂[cmp][i] = f <$> rtr₁[cmp][i]
+theorem obj?_updated : (LawfulUpdate cpt i f rtr₁ rtr₂) → rtr₂[cpt][i] = f <$> rtr₁[cpt][i]
   | update u => u.obj?_updated
   | notMem h e => by subst e; have h := member_isEmpty_obj?_none h; simp at h; simp [h]
 
@@ -264,18 +262,19 @@ namespace LawfulUpdatable
 
 variable [Indexable α] {rtr : α}
 
-theorem obj?_preserved {cmp f} (h : c ≠ cmp ∨ j ≠ i) : (update rtr cmp i f)[c][j] = rtr[c][j] :=
-  lawful rtr cmp i f |>.obj?_preserved h
+theorem obj?_preserved (h : c ≠ cpt ∨ j ≠ i) : (update rtr cpt i f)[c][j] = rtr[c][j] :=
+  lawful rtr cpt i f |>.obj?_preserved h
 
-theorem obj?_preserved_cmp {cmp f} (h : c ≠ cmp := by exact (nomatch ·)) : (update rtr cmp i f)[c][j] = rtr[c][j] :=
+theorem obj?_preserved_cpt (h : c ≠ cpt := by exact (nomatch ·)) : 
+    (update rtr cpt i f)[c][j] = rtr[c][j] :=
   obj?_preserved $ .inl h
 
-theorem obj?_preserved_id {cmp f} {c : Component.Valued} (h : j ≠ i) : 
-    (update rtr cmp i f)[c][j] = rtr[c][j] :=
+theorem obj?_preserved_id {c : Component.Valued} (h : j ≠ i) : 
+    (update rtr cpt i f)[c][j] = rtr[c][j] :=
   obj?_preserved $ .inr h
 
-theorem obj?_updated {rtr : α} {cmp i f} : (update rtr cmp i f)[cmp][i] = f <$> rtr[cmp][i] :=
-  lawful rtr cmp i f |>.obj?_updated
+theorem obj?_updated {rtr : α} : (update rtr cpt i f)[cpt][i] = f <$> rtr[cpt][i] :=
+  lawful rtr cpt i f |>.obj?_updated
 
 end LawfulUpdatable
 
@@ -286,16 +285,15 @@ variable [Indexable α] {rtr₁ : α}
 theorem obj?_rcn_eq (e : rtr₁ ≈ rtr₂) : rtr₁[.rcn] = rtr₂[.rcn] :=
   sorry
 
-theorem mem_obj?_ids_iff {cmp i} (e : rtr₁ ≈ rtr₂) : 
-    (i ∈ rtr₁[cmp].ids) ↔ (i ∈ rtr₂[cmp].ids) := by
+theorem mem_obj?_ids_iff {i} (e : rtr₁ ≈ rtr₂) : (i ∈ rtr₁[cpt].ids) ↔ (i ∈ rtr₂[cpt].ids) := by
   sorry
 
 theorem obj?_rtr_equiv (e : rtr₁ ≈ rtr₂) (h₁ : rtr₁[.rtr][i] = some n₁) (h₂ : rtr₂[.rtr][i] = some n₂) : 
     n₁ ≈ n₂ := by
   sorry
 
-theorem obj?_some_iff {cmp i} (e : rtr₁ ≈ rtr₂) :
-    (∃ o₁, rtr₁[cmp][i] = some o₁) ↔ (∃ o₂, rtr₂[cmp][i] = some o₂) := 
+theorem obj?_some_iff (e : rtr₁ ≈ rtr₂) :
+    (∃ o₁, rtr₁[cpt][i] = some o₁) ↔ (∃ o₂, rtr₂[cpt][i] = some o₂) := 
   sorry
 
 end Equivalent
