src/ReactorModel/Objects/Reactor/ReactorType/Updatable.lean
@@ -9,57 +9,57 @@ namespace ReactorType
 variable [ReactorType α] [ReactorType β] in section
 
 -- TODO: Find a better name for this.
-def RootEqualUpTo (cmp : Component) (i : ID) (rtr₁ rtr₂ : α) : Prop :=
-  ∀ {c j}, (c ≠ cmp ∨ j ≠ i) → cmp? c rtr₁ j = cmp? c rtr₂ j
+def RootEqualUpTo (cpt : Component) (i : ID) (rtr₁ rtr₂ : α) : Prop :=
+  ∀ {c j}, (c ≠ cpt ∨ j ≠ i) → cpt? c rtr₁ j = cpt? c rtr₂ j
 
-theorem RootEqualUpTo.mem_ids_iff {cmp} {rtr₁ : α} (e : RootEqualUpTo cmp i rtr₁ rtr₂) 
-    (h : c ≠ cmp ∨ j ≠ i) : j ∈ (cmp? c rtr₁).ids ↔ j ∈ (cmp? c rtr₂).ids := by
+theorem RootEqualUpTo.mem_ids_iff {rtr₁ : α} (e : RootEqualUpTo cpt i rtr₁ rtr₂) 
+    (h : c ≠ cpt ∨ j ≠ i) : j ∈ (cpt? c rtr₁).ids ↔ j ∈ (cpt? c rtr₂).ids := by
   simp [Partial.mem_ids_iff]
   exact ⟨(e h ▸ ·), (e h ▸ ·)⟩   
 
 -- Note: Without ID-uniqueness this can be satisfied by updating exactly one of the occurrences of
 --       the target. Since we have a choice of which target we update, this type isn't a `Prop`. 
 --       (We need to be able to eliminate into `Type` in `Member.fromLawfulUpdate`).
-inductive LawfulMemUpdate (cmp : Component.Valued) (i : ID) (f : cmp.type → cmp.type) : α → α → Type
+inductive LawfulMemUpdate (cpt : Component.Valued) (i : ID) (f : cpt.type → cpt.type) : α → α → Type
   | final : 
-    (RootEqualUpTo cmp i rtr₁ rtr₂) → (cmp? cmp rtr₁ i = some o) → (cmp? cmp rtr₂ i = f o) → 
-    LawfulMemUpdate cmp i f rtr₁ rtr₂
+    (RootEqualUpTo cpt i rtr₁ rtr₂) → (cpt? cpt rtr₁ i = some o) → (cpt? cpt rtr₂ i = f o) → 
+    LawfulMemUpdate cpt i f rtr₁ rtr₂
   | nest : 
-    (RootEqualUpTo .rtr j rtr₁ rtr₂) → (cmp? .rtr rtr₁ j = some n₁) → (cmp? .rtr rtr₂ j = some n₂) → 
-    (LawfulMemUpdate cmp i f n₁ n₂) → LawfulMemUpdate cmp i f rtr₁ rtr₂
+    (RootEqualUpTo .rtr j rtr₁ rtr₂) → (cpt? .rtr rtr₁ j = some n₁) → (cpt? .rtr rtr₂ j = some n₂) → 
+    (LawfulMemUpdate cpt i f n₁ n₂) → LawfulMemUpdate cpt i f rtr₁ rtr₂
 
 -- Note: This isn't a `Prop` because of the explanation on `LawfulMemUpdate`.
-inductive LawfulUpdate (cmp : Component.Valued) (i : ID) (f : cmp.type → cmp.type) (rtr₁ rtr₂ : α)
-  | update (u : LawfulMemUpdate cmp i f rtr₁ rtr₂)
-  | notMem (h : IsEmpty $ Member cmp i rtr₁) (eq : rtr₁ = rtr₂)
+inductive LawfulUpdate (cpt : Component.Valued) (i : ID) (f : cpt.type → cpt.type) (rtr₁ rtr₂ : α)
+  | update (u : LawfulMemUpdate cpt i f rtr₁ rtr₂)
+  | notMem (h : IsEmpty $ Member cpt i rtr₁) (eq : rtr₁ = rtr₂)
 
-theorem RootEqualUpTo.lift [l : LawfulCoe α β] {cmp i} {rtr₁ rtr₂ : α} 
-    (e : RootEqualUpTo cmp i (rtr₁ : β) (rtr₂ : β)) : RootEqualUpTo cmp i rtr₁ rtr₂ := by
+theorem RootEqualUpTo.lift [l : LawfulCoe α β] {rtr₁ rtr₂ : α} 
+    (e : RootEqualUpTo cpt i (rtr₁ : β) (rtr₂ : β)) : RootEqualUpTo cpt i rtr₁ rtr₂ := by
   intro c j h
   have he := e h
-  cases h₁ : cmp? c (rtr₁ : β) j <;> cases h₂ : cmp? c (rtr₂ : β) j <;> simp_all
-  case none.none => simp [l.lift_cmp?_eq_none _ h₁, l.lift_cmp?_eq_none _ h₂]
+  cases h₁ : cpt? c (rtr₁ : β) j <;> cases h₂ : cpt? c (rtr₂ : β) j <;> simp_all
+  case none.none => simp [l.lift_cpt?_eq_none _ h₁, l.lift_cpt?_eq_none _ h₂]
   case some.some => 
     cases c <;> try cases ‹Reactor.Component.Valued› 
-    all_goals try simp [l.lift_cmp?_eq_some _ h₁, l.lift_cmp?_eq_some _ h₂]
+    all_goals try simp [l.lift_cpt?_eq_some _ h₁, l.lift_cpt?_eq_some _ h₂]
     case rtr =>
       have ⟨_, _, h₁'⟩ := l.lift_nest_eq_some h₁
       have ⟨_, _, h₂'⟩ := l.lift_nest_eq_some h₂
       subst h₁'
-      simp [l.lift_cmp?_eq_some _ h₁, l.lift_cmp?_eq_some _ h₂]
+      simp [l.lift_cpt?_eq_some _ h₁, l.lift_cpt?_eq_some _ h₂]
 
-def LawfulMemUpdate.lift [c : LawfulCoe α β] {rtr₁ rtr₂ : α} {cmp i f} :
-    (LawfulMemUpdate cmp i f (rtr₁ : β) (rtr₂ : β)) → LawfulMemUpdate cmp i f rtr₁ rtr₂
+def LawfulMemUpdate.lift [c : LawfulCoe α β] {rtr₁ rtr₂ : α} :
+    (LawfulMemUpdate cpt i f (rtr₁ : β) (rtr₂ : β)) → LawfulMemUpdate cpt i f rtr₁ rtr₂
   | final e h₁ h₂ (o := o) => 
-    have h₁ : cmp? cmp rtr₁ i = some o     := by cases cmp <;> exact c.lift_cmp?_eq_some _ h₁
-    have h₂ : cmp? cmp rtr₂ i = some (f o) := by cases cmp <;> exact c.lift_cmp?_eq_some _ h₂
+    have h₁ : cpt? cpt rtr₁ i = some o     := by cases cpt <;> exact c.lift_cpt?_eq_some _ h₁
+    have h₂ : cpt? cpt rtr₂ i = some (f o) := by cases cpt <;> exact c.lift_cpt?_eq_some _ h₂
     .final e.lift h₁ h₂
   | nest (n₁ := n₁) (n₂ := n₂) e h₁ h₂ u (j := j) => 
     have o₁ := c.lift_nest_eq_some h₁
     have o₂ := c.lift_nest_eq_some h₂
     have ⟨h₁, h₁'⟩ := o₁.choose_spec
     have ⟨h₂, h₂'⟩ := o₂.choose_spec 
-    let u' : LawfulMemUpdate cmp i f (o₁.choose : β) (o₂.choose : β) := cast (by simp [h₁', h₂']) u
+    let u' : LawfulMemUpdate cpt i f (o₁.choose : β) (o₂.choose : β) := cast (by simp [h₁', h₂']) u
     .nest e.lift h₁ h₂ u'.lift
 termination_by lift u => sizeOf u
 decreasing_by simp_wf; have h : sizeOf u' = sizeOf u := (by congr; apply cast_heq); simp [h]
@@ -75,8 +75,8 @@ decreasing_by simp_wf; have h : sizeOf u' = sizeOf u := (by congr; apply cast_he
 --
 -- ... there's something functorial about this. The `lift` looks like a functor's `map` over `u`.
 -- Figure out if there's a way of modelling some part of this as a functor. 
-def LawfulUpdate.lift [c : LawfulCoe α β] {rtr₁ rtr₂ : α} {cmp i f} :
-    (LawfulUpdate cmp i f (rtr₁ : β) (rtr₂ : β)) → LawfulUpdate cmp i f rtr₁ rtr₂
+def LawfulUpdate.lift [c : LawfulCoe α β] {rtr₁ rtr₂ : α} :
+    (LawfulUpdate cpt i f (rtr₁ : β) (rtr₂ : β)) → LawfulUpdate cpt i f rtr₁ rtr₂
   | update u => update u.lift
   | notMem h eq =>  
     let u := notMem (byContradiction (h.false $ not_isEmpty_iff.mp · |>.some.fromLawfulCoe)) rfl
@@ -85,20 +85,20 @@ def LawfulUpdate.lift [c : LawfulCoe α β] {rtr₁ rtr₂ : α} {cmp i f} :
 end
 
 class Updatable (α) extends ReactorType.WellFounded α where
-  update : α → (cmp : Component.Valued) → ID → (cmp.type → cmp.type) → α  
+  update : α → (cpt : Component.Valued) → ID → (cpt.type → cpt.type) → α  
     
 class LawfulUpdatable (α) extends Updatable α where 
-  lawful : ∀ rtr cmp i f, LawfulUpdate cmp i f rtr (update rtr cmp i f)      
+  lawful : ∀ rtr cpt i f, LawfulUpdate cpt i f rtr (update rtr cpt i f)      
 
 scoped macro "lawfulUpdatableCoe_update_coe_comm_proof" : tactic =>
   `(tactic| simp [Updatable.update, Coe.coe])
 
 class LawfulUpdatableCoe (α β) [a : Updatable α] [b : Updatable β] extends LawfulCoe α β where
   update_coe_comm : 
-    ∀ {rtr cmp i f}, b.update (coe rtr) cmp i f = coe (a.update rtr cmp i f) := by 
+    ∀ {rtr cpt i f}, b.update (coe rtr) cpt i f = coe (a.update rtr cpt i f) := by 
       lawfulUpdatableCoe_update_coe_comm_proof
 
 instance [Updatable α] [LawfulUpdatable β] [c : LawfulUpdatableCoe α β] : LawfulUpdatable α where
-  lawful rtr cmp i f := c.update_coe_comm ▸ LawfulUpdatable.lawful (rtr : β) cmp i f |>.lift 
+  lawful rtr cpt i f := c.update_coe_comm ▸ LawfulUpdatable.lawful (rtr : β) cpt i f |>.lift 
 
 end ReactorType
